[Parikh] some basic lemmas about regular functions

Parikh/Parikh.thy
@@ -46,23 +46,118 @@ primrec subst :: "'a lfun \<Rightarrow> (nat \<Rightarrow> 'a lfun) \<Rightarrow
 section \<open>Regular functions\<close>
 
 inductive regular_fun :: "'a lfun \<Rightarrow> bool" where
-  "regular_fun (V _)" |
-  "regular_lang l \<Longrightarrow> regular_fun (N l)" |
-  "\<lbrakk> regular_fun f; regular_fun g \<rbrakk> \<Longrightarrow> regular_fun (Union2 f g)" |
-  "\<lbrakk> regular_fun f; regular_fun g \<rbrakk> \<Longrightarrow> regular_fun (Conc f g)" |
-  "regular_fun f \<Longrightarrow> regular_fun (Star f)"
+  Variable:    "regular_fun (V _)" |
+  Const:       "regular_lang l \<Longrightarrow> regular_fun (N l)" |
+  Union2:      "\<lbrakk> regular_fun f; regular_fun g \<rbrakk> \<Longrightarrow> regular_fun (Union2 f g)" |
+  Conc:        "\<lbrakk> regular_fun f; regular_fun g \<rbrakk> \<Longrightarrow> regular_fun (Conc f g)" |
+  Star:        "regular_fun f \<Longrightarrow> regular_fun (Star f)"
+
+declare regular_fun.intros [intro]
+inductive_cases ConstE [elim]:       "regular_fun (N l)"
+inductive_cases Union2E [elim]:      "regular_fun (Union2 f g)"
+inductive_cases ConcE [elim]:        "regular_fun (Conc f g)"
+inductive_cases StarE [elim]:        "regular_fun (Star f)"
+
+
+lemma countable_union_finally_empty:
+  assumes "\<forall>j>i. f j = {}"
+  shows "(\<Union>j. f j) = (\<Union>j\<le>i. f j)"
+  sorry
+
+
+lemma finite_union_regular:
+  assumes "\<forall>j\<le>i. regular_fun (f j)"
+      and "\<forall>j>i. f j = N {}"
+    shows "\<exists>g. regular_fun g \<and> (\<forall>s. eval (UnionC f) s = eval g s)"
+using assms proof (induction i arbitrary: f)
+  case 0
+  then have "eval (UnionC f) s = eval (f 0) s" for s
+    using countable_union_finally_empty[of 0 "\<lambda>j. eval (f j) s"] by simp
+  with "0.prems" show ?case by blast
+next
+  case (Suc i)
+  let ?f' = "(\<lambda>j. if j \<le> i then f j else N {})"
+  from Suc obtain g' where "regular_fun g' \<and> (\<forall>s. eval (UnionC ?f') s = eval g' s)" by fastforce
+  moreover with Suc.prems have "eval (UnionC f) s = eval (Union2 g' (f (Suc i))) s" for s
+    using countable_union_finally_empty[of "Suc i" "\<lambda>j. eval (f j) s"]
+          countable_union_finally_empty[of i "\<lambda>j. eval (?f' j) s"]
+    by (simp add: atMost_Suc sup_commute)
+  ultimately show ?case using Suc.prems by blast
+qed
+
 
 lemma regular_fun_regular:
   assumes "regular_fun f"
-      and "n \<in> vars f \<Longrightarrow> regular_lang (s n)"
+      and "\<And>n. n \<in> vars f \<Longrightarrow> regular_lang (s n)"
     shows "regular_lang (eval f s)"
-  sorry
+using assms proof (induction rule: regular_fun.induct)
+  case (Union2 f g)
+  then obtain r1 r2 where "Regular_Exp.lang r1 = eval f s \<and> Regular_Exp.lang r2 = eval g s" by auto
+  then have "Regular_Exp.lang (Plus r1 r2) = eval (Union2 f g) s" by simp
+  then show ?case by blast
+next
+  case (Conc f g)
+  then obtain r1 r2 where "Regular_Exp.lang r1 = eval f s \<and> Regular_Exp.lang r2 = eval g s" by auto
+  then have "Regular_Exp.lang (Times r1 r2) = eval (Conc f g) s" by simp
+  then show ?case by blast
+next
+  case (Star f)
+  then obtain r  where "Regular_Exp.lang r = eval f s" by auto
+  then have "Regular_Exp.lang (Regular_Exp.Star r) = eval (Star f) s" by simp
+  then show ?case by blast
+qed auto
+
 
 lemma regular_fun_mono:
   assumes "regular_fun f"
+  shows "mono (eval f)"
+using assms proof (induction rule: regular_fun.induct)
+  case (Variable uu)
+  then show ?case by (simp add: le_funD ord.mono_on_def)
+next
+  case (Const l)
+  then show ?case by (simp add: ord.mono_on_def)
+next
+  case (Union2 f g)
+  then show ?case by (smt (verit, best) eval.simps(3) ord.mono_on_def sup_mono)
+next
+  case (Conc f g)
+  then show ?case by (simp add: conc_mono ord.mono_on_def)
+next
+  case (Star f)
+  then show ?case
+    by (smt (verit, best) dual_order.trans eval.simps(6) in_star_iff_concat monotone_on_def subsetI)
+qed
+
+
+(*lemma regular_fun_mono:
+  assumes "regular_fun f"
       and "\<forall>i. s i \<subseteq> s' i"
     shows "eval f s \<subseteq> eval f s'"
-  sorry
+using assms proof (induction rule: regular_fun.induct)
+  case (Variable uu)
+  then show ?case by auto
+next
+  case (Const l)
+  then show ?case by auto
+next
+  case (Union2 f g)
+  then show ?case by auto
+next
+  case (Conc f g)
+  then show ?case by fastforce
+next
+  case (Star f)
+  have "\<And>w. w \<in> star (eval f s) \<Longrightarrow> w \<in> star (eval f s')"
+  proof -
+    fix w
+    assume "w \<in> star (eval f s)"
+    then obtain n where "w \<in> (eval f s) ^^ n" using star_pow by auto
+    with Star have "w \<in> (eval f s') ^^ n" using funpow_mono sorry
+    show "w \<in> star (eval f s')" sorry
+  qed
+  then show ?case sorry
+qed*)
 
 
 section \<open>Parikh image\<close>
@@ -83,8 +178,11 @@ section \<open>systems of equations\<close>
 type_synonym 'a eq_sys = "'a lfun list"
 
 (* sys independent on variables \<le> n *)
-definition indep :: "'a eq_sys \<Rightarrow> nat \<Rightarrow> bool" where
-  "indep sys n \<equiv> \<forall>eq \<in> set sys. \<forall>x \<in> vars eq. x > n"
+definition indep_ub :: "'a eq_sys \<Rightarrow> nat \<Rightarrow> bool" where
+  "indep_ub sys n \<equiv> \<forall>eq \<in> set sys. \<forall>x \<in> vars eq. x > n"
+
+definition indep_lb :: "'a eq_sys \<Rightarrow> nat \<Rightarrow> bool" where
+  "indep_lb sys n \<equiv> \<forall>eq \<in> set sys. \<forall>x \<in> vars eq. x < n"
 
 definition solves_ineq_sys :: "'a eq_sys \<Rightarrow> 'a state \<Rightarrow> bool" where
   "solves_ineq_sys sys s \<equiv> \<forall>i < length sys. eval (sys ! i) s \<subseteq> s i"
@@ -102,7 +200,7 @@ definition sys_subst :: "'a eq_sys \<Rightarrow> (nat \<Rightarrow> 'a lfun) \<R
   "sys_subst sys s \<equiv> map (\<lambda>eq. subst eq s) sys"
 
 definition partial_sol :: "'a eq_sys \<Rightarrow> 'a eq_sys \<Rightarrow> bool" where
-  "partial_sol sys sol \<equiv> length sol = length sys \<and> indep sol (length sys - 1)
+  "partial_sol sys sol \<equiv> length sol = length sys \<and> indep_ub sol (length sys - 1)
                   \<and> (\<forall>s. solves_eq_sys_comm (sys_subst sys (\<lambda>i. if i < length sys then sol ! i else V i)) s)"
 
 
@@ -117,7 +215,7 @@ definition g :: "'a eq_sys \<Rightarrow> nat \<Rightarrow> 'a lfun" where
 
 lemma lemma_paper:
   assumes "\<forall>eq \<in> set f_sys. regular_fun eq"
-    shows "\<exists>g_sys. length g_sys = length f_sys \<and> indep g_sys (length f_sys - 1)
+    shows "\<exists>g_sys. length g_sys = length f_sys \<and> indep_ub g_sys (length f_sys - 1)
                 \<and> (solves_ineq_sys f_sys s \<longrightarrow> solves_ineq_sys g_sys s)
                 \<and> (solves_eq_sys g_sys s \<longrightarrow> solves_eq_sys f_sys s)"
   sorry
@@ -141,7 +239,7 @@ lemma theorem_paper:
 
 lemma
   assumes "\<forall>eq \<in> set f_sys. regular_fun eq"
-      and "\<forall>eq \<in> set f_sys. \<forall>x \<in> vars eq. x < length f_sys"
+      and "indep_lb f_sys (length f_sys)"
     shows "\<exists>s. (\<forall>i. regular_lang (s i)) \<and> solves_eq_sys_comm f_sys s
           \<and> (\<forall>s'. solves_eq_sys_comm f_sys s' \<longrightarrow> (\<forall>i. parikh_img (s' i) \<subseteq> parikh_img (s i)))"
   sorry
